Weakened the definition of registered.

src/DependencyStateImpl.v
@@ -1,3 +1,5 @@
+Set Implicit Arguments.
+
 Require Import Brenner.ResourceDependency.
 Require Import Brenner.DependencyState.
 Require Import Brenner.Vars.
@@ -12,7 +14,8 @@ Require Import Aniceto.Project.
 Require Import Aniceto.Map.
 Require Import Aniceto.Set.
 
-Set Implicit Arguments.
+Module I := Project Map_EVT Set_TID.
+Module W := Project Map_TID Set_EVT.
 
 (** We build the phaser map of waiting tasks to be constituted by all
    blocked tasks in state [s]. *)
@@ -94,6 +97,8 @@ Qed.
 
 End Basic.
 
+Section Props.
+
 Definition blocked (s:state) (e:(tid*prog)) : option event :=
   let (t, prg) := e in
   match prg with
@@ -111,16 +116,15 @@ Definition blocked (s:state) (e:(tid*prog)) : option event :=
     | _ => None
   end.
 
-Definition get_blocked s :=
-  filter (fun e:(tid*prog) =>
+Definition wait_on s : list (tid * event) :=
+  List.omap (fun e =>
     match blocked s e with
-      | Some _ => true
-      | None => false
-    end)
-  (Map_TID.elements (get_tasks s)).
+    | Some r => Some (fst e,r)
+    | None => None
+    end
+  ) (Map_TID.elements (get_tasks s)).
 
-
-Lemma blocked_inv_1:
+Let blocked_inv_1:
   forall s t p n r prg,
   blocked s (t, pcons (Await p n) prg) =
        Some r ->
@@ -137,7 +141,7 @@ Proof.
   + inversion H.
 Qed.
 
-Lemma blocked_inv_2:
+Let blocked_inv_2:
   forall s t p n prg,
   blocked s (t, pcons (Await p n) prg) = None ->
   ~ Map_PHID.In p (get_phasers s).
@@ -152,7 +156,7 @@ Proof.
     assumption.
 Qed.
 
-Lemma blocked_inv_3:
+Let blocked_inv_3:
   forall s t r prg r',
   blocked s (t, pcons (Await (get_phaser r) (get_phase r)) prg) =
        Some r' ->
@@ -165,7 +169,7 @@ Proof.
   auto.
 Qed.
 
-Lemma blocked_spec:
+Let blocked_spec:
   forall s t prg r,
   blocked s (t, prg) = Some r <->
   (exists prg',  prg = (pcons (Await (get_phaser r) (get_phase r)) prg'))
@@ -215,115 +219,141 @@ Proof.
   + inversion H1.
 Qed.
 
-Lemma get_blocked_spec_1:
-  forall t prg s,
-  In (t, prg) (get_blocked s) ->
-  exists e, blocked s (t, prg) = Some e /\ WaitsFor s t e.
+Let waits_for_def:
+  forall p e s t,
+  Map_PHID.In (get_phaser e) (get_phasers s) ->
+  Map_TID.MapsTo t (pcons (Await (get_phaser e) (get_phase e)) p) (get_tasks s) ->
+  WaitsFor s t e.
 Proof.
-  unfold get_blocked.
   intros.
-  rewrite filter_In in H.
-  intros.
-    destruct H.
-    apply Map_TID_Extra.in_elements_impl_maps_to in H.
-    remember (blocked s (t, prg)) as o.
-    symmetry in Heqo.
-    destruct o.
-    + exists e.
-      intuition.
-      apply blocked_spec in Heqo.
-      unfold WaitsFor.
-      destruct Heqo as ((prg', Heq), Hin).
-      intuition.
-      subst.
-      exists prg'.
-      intuition.
-    + inversion H0.
+  unfold WaitsFor.
+  eauto.
 Qed.
 
-Lemma get_blocked_spec_2:
-  forall s t prg e,
-  blocked s (t, prg) = Some e ->
-  Map_TID.MapsTo t prg (get_tasks s) ->
-  In (t, prg) (get_blocked s).
+Let wait_on_1:
+  forall t s e,
+  In (t, e) (wait_on s) ->
+  WaitsFor s t e.
 Proof.
+  unfold wait_on.
   intros.
-  rewrite blocked_spec in H.
-  unfold get_blocked.
-  rewrite filter_In.
-  remember (blocked s (t, prg)).
-  destruct H as ((prg', Heq), Hin).
-  rewrite <- Map_TID_Extra.maps_to_iff_in_elements.
-  + intuition.
-    destruct o.
-    trivial.
+  apply List.in_omap_2 in H.
+  destruct H as ((x,p), (Hi, Hb)).
+  apply Map_TID_Extra.in_elements_impl_maps_to in Hi.
+  remember (blocked _ _) as o.
+  symmetry in Heqo.
+  destruct o. {
+    apply blocked_spec in Heqo.
+    inversion Hb; subst; clear Hb.
+    destruct Heqo as ((?,?), ?).
     subst.
-    inversion Heqo.
-    remember (Map_PHID.find (elt:=Phaser.phaser) (get_phaser e) (get_phasers s)) as o'.
-    symmetry in Heqo'.
-    destruct o'.
-    inversion H1.
-    apply Map_PHID_Facts.not_find_in_iff in Heqo'.
-    contradiction Heqo'.
-  + auto.
+    eauto using waits_for_def.
+  }
+  inversion Hb.
 Qed.
 
-Definition gen_wedges s : list (tid*event) :=
-  flat_map
-  (fun (e:(tid*prog))  =>
-    match (blocked s e) with
-      | Some r => (fst e, r) :: nil
-      | None => nil
-    end)
-  (get_blocked s).
-
-Lemma gen_wedges_spec:
-  forall e t s,
-  In (t, e) (gen_wedges s) <-> WaitsFor s t e.
+Let wait_on_2:
+  forall t s e,
+  WaitsFor s t e ->
+  In (t, e) (wait_on s).
 Proof.
-  intros.
-  unfold gen_wedges.
-  rewrite in_flat_map.
-  split.
-  - intros.
-    destruct H as ((t',prg'), (Hin, Hin')).
-    apply get_blocked_spec_1 in Hin.
-    destruct Hin as (r', (Hb, Hb')).
-    remember (blocked s (t', prg')) as o.
-    destruct o.
-    + inversion Hb; subst; clear Hb.
-      apply in_inv in Hin'.
-      destruct Hin'.
-      simpl in H; inversion H; subst; clear H.
-      assumption.
-      inversion H.
-    + inversion Hb.
-  - intros.
-    destruct H as (prg, (Hin, Hpin)).
-    remember ((pcons (Await (get_phaser e) (get_phase e)) prg)) as prg'.
-    exists (t, prg').
-    remember (blocked s (t, prg')) as o.
-    destruct o.
+  unfold wait_on; intros.
+  destruct H as (p, (?,?)).
+    remember (pcons _ _) as p'.
+    apply List.in_omap_1 with (x:=(t,p')). {
+      rewrite <- Map_TID_Extra.maps_to_iff_in_elements; auto.
+    }
+    remember (blocked _ _).
     symmetry in Heqo.
-    split.
-    + apply get_blocked_spec_2 with (e:=e0).
-      assumption.
-      assumption.
-    + subst.
-      apply blocked_inv_1 in Heqo.
-      destruct e0; inversion Heqo; subst; clear Heqo.
-      destruct e.
-      simpl in *.
-      auto.
-    + subst.
-      symmetry in Heqo.
-      apply blocked_inv_2 in Heqo.
-      contradiction Heqo.
+    destruct o. {
+      apply blocked_spec in Heqo.
+      destruct Heqo as ((p'',Heq), ?).
+      subst.
+      inversion Heq; subst; clear Heq.
+      destruct e, e0; simpl in *.
+      subst.
+      trivial.
+    }
+    subst; apply blocked_inv_2 in Heqo.
+    contradiction.
 Qed.
 
-Module W := Project Map_TID Set_EVT.
+Let wait_on_spec:
+  forall t s e,
+  In (t, e) (wait_on s) <->
+  WaitsFor s t e.
+Proof.
+  split; eauto.
+Qed.
 
-Lemma tid_eq_subst:
+Definition registered s : list (tid*event) :=
+  let on_registered (p:phid*Phaser.phaser) :=
+    let (p, ph) := p in
+    let handle (e:tid*nat) :=
+      let (t, n) := e in
+      match Map_TID.find t (get_tasks s) with
+      | Some _ => Some (t, (p, n))
+      | _ => None
+      end
+    in
+    List.omap handle (Map_TID.elements ph)
+  in
+  flat_map on_registered (Map_PHID.elements (get_phasers s)).
+
+Let registered_1:
+  forall t e s,
+  In (t, e) (registered s) ->
+  Registered s t e.
+Proof.
+  unfold registered; intros.
+  apply in_flat_map in H.
+  destruct H as ((p,ph), (Hi, Hp)).
+  apply Map_PHID_Extra.maps_to_iff_in_elements in Hi; auto.
+  apply List.in_omap_2 in Hp.
+  destruct Hp as ((t',n), (Hp,Hx)).
+  apply Map_TID_Extra.maps_to_iff_in_elements in Hp; auto.
+  destruct (Map_TID_Extra.find_rw t' (get_tasks s)) as [(R,Hy)|(p',(R,?))]. {
+    rewrite R in *.
+    inversion Hx.
+  }
+  rewrite R in *.
+  inversion Hx; subst; clear Hx.
+  eauto using registered_def, Map_TID_Extra.mapsto_to_in.
+Qed.
+
+Let registered_2:
+  forall t e s,
+  Registered s t e ->
+  In (t, e) (registered s).
+Proof.
+  unfold registered; intros.
+  apply in_flat_map.
+  destruct H as (ph, (Hp,(Ht,Hi))).
+  exists ((get_phaser e),ph).
+  split. {
+    rewrite <- Map_PHID_Extra.maps_to_iff_in_elements; auto.
+  }
+  apply List.in_omap_1 with (x:=(t, (get_phase e))); eauto. {
+    rewrite <- Map_TID_Extra.maps_to_iff_in_elements; auto.
+  }
+  destruct (Map_TID_Extra.find_rw t (get_tasks s)) as [(R,Hy)|(p',(R,?))];
+  rewrite R in *; clear R. {
+    contradiction.
+  }
+  destruct e; simpl in *.
+  trivial.
+Qed.
+
+Let registered_spec:
+  forall t e s,
+  In (t, e) (registered s) <->
+  Registered s t e.
+Proof.
+  split; eauto.
+  
+Qed.
+
+Let tid_eq_subst:
   forall (e1 e2:tid), Map_TID.E.eq e1 e2 <-> e1 = e2.
 Proof.
   intros.
@@ -331,7 +361,7 @@ Proof.
   split; auto.
 Qed.
 
-Lemma evt_eq_subst:
+Let evt_eq_subst:
   forall (e1 e2:event), Map_EVT.E.eq e1 e2 <-> e1 = e2.
 Proof.
   intros.
@@ -352,9 +382,9 @@ Proof.
 auto.
 Qed.
 
-Definition to_waits s := W.unproject tid_eq_helper (gen_wedges s).
+Definition to_waits s := W.unproject tid_eq_helper (wait_on s).
 
-Lemma waits_total:
+Let waits_total:
   forall (s:state),
   exists (w:waits), W_of s w.
 Proof.
@@ -365,268 +395,100 @@ Proof.
   split.
   - intros.
     apply W.unproject_spec in H.
-    apply gen_wedges_spec in H.
+    apply wait_on_spec in H.
     assumption.
     apply evt_eq_subst.
   - intros.
-    apply gen_wedges_spec in H.
+    apply wait_on_spec in H.
     apply W.unproject_spec.
     apply evt_eq_subst.
     assumption.
 Qed.
 
-Definition is_blocked (s:state) (t:tid) : bool :=
-  match Map_TID.find t (get_tasks s) with
-    | Some prg =>
-      match blocked s (t, prg) with
-        | Some _ => true
-        | _ => false
-      end
-    | _ => false
-  end.
-
-Lemma is_blocked_spec:
-  forall s t,
-  is_blocked s t = true <-> exists e, WaitsFor s t e.
+Let prec_dec e e' :
+  { prec e e' } + { ~ prec e e'}.
 Proof.
-  intros.
-  unfold is_blocked.
-  remember (Map_TID.find (elt:=prog) t (get_tasks s)) as of.
-  symmetry in Heqof.
-  unfold WaitsFor.
-  destruct of.
-  + apply Map_TID_Facts.find_mapsto_iff in Heqof.
-    remember (blocked s (t, p)) as ob.
-    symmetry in Heqob.
-    destruct ob.
-    * apply blocked_spec in Heqob.
-      intuition.
-      destruct H as (prg', Heq).
-      exists e.
-      exists prg'.
-      subst.
+  unfold prec.
+  destruct (PHID.eq_dec (get_phaser e) (get_phaser e')). {
+    destruct (lt_dec (get_phase e) (get_phase e')). {
       auto.
-    * intuition.
-      inversion H.
-      destruct H as (r, (prg, (Hmt, Hpin))).
-      apply Map_TID_Facts.MapsTo_fun with (e:=p) in Hmt.
-      subst.
-      apply blocked_inv_2 in Heqob.
-      contradiction Heqob.
-      auto.
-  + intuition.
-    inversion H.
-    destruct H as (r, (prg, (Hmt, Hpin))).
-    apply Map_TID_Facts.not_find_in_iff in Heqof.
-    apply Map_TID_Extra.mapsto_to_in in Hmt.
-    contradiction Heqof.
-Qed.
+    }
+    right.
+    unfold not; intros N.
+    destruct N.
+    contradiction.
+  }
+  right.
+  unfold not; intros N.
+  destruct N.
+  contradiction.
+Defined.
 
-Lemma is_blocked_from_prop:
-  forall s t r,
-   WaitsFor s t r ->
-   is_blocked s t = true.
-Proof.
-  intros.
-  rewrite is_blocked_spec.
-  exists r; assumption.
-Qed.
+Definition impeded_by s :=
+  let es := List.map (fun p => snd p) (wait_on s) in
+  let handle_entry (e:event) (p:tid*event) :=
+    let (t, e') := p in
+    if prec_dec e' e then Some (e, t)
+    else None
+  in
+  let reg := registered s in
+  let handle e :=
+    List.omap (handle_entry e) reg
+  in
+  flat_map handle es.
 
-Definition blocks (s:state) (e:event) : list tid :=
-  match Map_PHID.find (get_phaser e) (get_phasers s) with
-    | Some ph =>
-        flat_map
-        (fun (p:tid*nat) =>
-          let (t, n) := p in
-          if lt_ge_dec n (get_phase e)
-          then if is_blocked s t then (t :: nil) else nil
-          else nil)
-        (Map_TID.elements ph)
-    | _ => nil
-  end.
-
-Lemma blocks_spec_1:
-  forall (s:state) (e:event) (t:tid) (t':tid),
-  In t (blocks s e) ->
-  WaitsFor s t' e ->
+Let impeded_by_1:
+  forall t e s,
+  In (e, t) (impeded_by s) ->
   Impedes s e t.
 Proof.
-  unfold blocks.
-  intros.
-  remember (Map_PHID.find (get_phaser e) (get_phasers s)) as of.
-  symmetry in Heqof.
-  destruct of.
-  - apply <- Map_PHID_Facts.find_mapsto_iff in Heqof.
-    rewrite in_flat_map in H.
-    destruct H as ((t'',n), (Hin, Hin')).
-    apply Map_TID_Extra.in_elements_impl_maps_to in Hin.
-    remember (is_blocked s t'') as o.
-    destruct (lt_ge_dec n (get_phase e)), o.
-    + destruct Hin'.
-      subst.
-      apply impedes_def with (t':=t') (e':=((get_phaser e), n)); repeat auto.
-      unfold Registered.
-      exists p.
-      simpl in *.
-      intuition.
-      symmetry in Heqo.
-      apply is_blocked_spec in Heqo.
-      assumption.
-      unfold prec.
-      auto.
-      inversion H.
-    + inversion Hin'.
-    + inversion Hin'.
-    + inversion Hin'.
-  - inversion H.
-Qed.
-
-Lemma blocks_spec_2:
-  forall (s:state) (e:event) (t:tid),
-  Impedes s e t ->
-  In t (blocks s e).
-Proof.
-  intros.
-  unfold blocks.
-  remember (Map_PHID.find (get_phaser e) (get_phasers s)) as of.
-  symmetry in Heqof.
-  destruct of.
-  + apply in_flat_map.
-    destruct H as ((t1, Ht1b), (r', ((ph, (Hmt, (Hmt', (r'', Hb)))), (Heq, Hlt)))).
-      destruct r' as (h', n').
-      destruct e as (h, n).
-      simpl in *; subst.
-      exists (t, n').
-      rename p into ph'.
-      apply Map_TID_Extra.maps_to_iff_in_elements in Hmt'.
-      apply Map_PHID_Facts.MapsTo_fun with (e:=ph') in Hmt.
-      subst.
-      intuition.
-      destruct (lt_ge_dec n' n).
-      remember (is_blocked s t) as b.
-      symmetry in Heqb.
-      destruct b.
-      apply in_eq.
-      apply is_blocked_from_prop in Hb.
-      rewrite Heqb in Hb.
-      inversion Hb.
-      apply Lt.lt_not_le in Hlt.
-      assert (n <= n').
-      auto.
-      contradiction Hlt.
-      apply Map_PHID_Facts.find_mapsto_iff in Heqof.
-      assumption.
-      auto.
-   + apply Map_PHID_Facts.not_find_in_iff in Heqof.
-     apply impedes_in_phasermap in H.
-     contradiction Heqof.
-Qed.
-
-Definition gen_tedges s : list (event*tid) :=
-  flat_map
-  (fun (edge:(tid*prog))  =>
-    match (blocked s edge) with
-      | Some e => map (fun t => (e, t)) (blocks s e)
-      | None => nil
-    end)
-  (get_blocked s).
-
-Lemma in_gen_tedges_to_blocks:
-  forall r t s,
-  In (r, t) (gen_tedges s) -> Impedes s r t.
-Proof.
-  intros.
-  unfold gen_tedges in *.
+  unfold impeded_by; intros.
   apply in_flat_map in H.
-  destruct H as ((t', prg), (Hinb, Hinr)).
-  remember (blocked s (t', prg)).
-  symmetry in Heqo.
-  destruct o.
-  + apply in_map_iff in Hinr.
-    destruct Hinr as (t'', (Heq, Himp)).
-    inversion Heq.
-    subst.
-    clear Heq.
-    apply blocks_spec_1 with (t':=t') in Himp.
-    assumption.
-    apply get_blocked_spec_1 in Hinb.
-    destruct Hinb as (r', (Hblocked, Hb)).
-    rewrite Heqo in Hblocked.
-    inversion Hblocked.
-    subst.
-    assumption.
-  + inversion Hinr.
+  destruct H as (e', (Hi, Hm)).
+  apply in_map_iff in Hi.
+  destruct Hi as ((t',e''), (?, Hi)).
+  simpl in *; subst.
+  apply wait_on_spec in Hi.
+  apply List.in_omap_2 in Hm.
+  destruct Hm as ((t'', e''), (Hr, Heq)).
+  apply registered_spec in Hr.
+  destruct (prec_dec e'' e'). {
+    inversion Heq; subst.
+    unfold Impedes; eauto.
+  }
+  inversion Heq.
 Qed.
 
-Lemma blocked_from_prop:
-  forall s t e,
-  WaitsFor s t e ->
-  exists prg, In (t, prg) (get_blocked s) /\
-  blocked s (t, prg) = Some e.
-Proof.
-  intros.
-  unfold WaitsFor in *.
-  destruct H as (prg, (Hmt, Hph)).
-  remember (pcons (Await (get_phaser e) (get_phase e)) prg) as prg'.
-  assert (Hn : blocked s (t, prg') = Some e).
-  apply blocked_spec.
-  intuition.
-  exists prg.
-  assumption.
-  exists prg'.
-  intuition.
-  apply get_blocked_spec_2 with (e:=e).
-  assumption.
-  assumption.
-Qed.
-
-Lemma blocks_to_in_gen_tedges:
-  forall s e t,
+Let impeded_by_2:
+  forall t e s,
   Impedes s e t ->
-  In (e, t) (gen_tedges s).
+  In (e, t) (impeded_by s).
 Proof.
   intros.
-  unfold gen_tedges.
-  apply in_flat_map.
-  assert (Hx := H).
-  destruct H as ((t', Hb), (e', (Hr,Hprec))).
-  destruct Hb as (prg, (Hb1,Hb2)).
-  remember (pcons (Await (get_phaser e) (get_phase e)) prg) as prg'.
-  exists (t', prg').
-  split.
-  + apply get_blocked_spec_2 with (e:=e).
-    * apply blocked_spec.
-      intuition.
-      exists prg.
-      assumption.
-    * assumption.
-  + remember (blocked s (t', prg')).
-    rewrite Heqprg' in Heqo.
-    symmetry in Heqo.
-    destruct o.
-    * apply in_map_iff.
-      exists t.
-      apply blocked_inv_3 in Heqo.
-      subst.
-      intuition.
-      apply blocks_spec_2.
-      assumption.
-    * apply blocked_inv_2 in Heqo.
-      contradiction Heqo.
+  unfold impeded_by.
+  rewrite in_flat_map.
+  exists e.
+  destruct H as ((t',Hw),(e',(Hr,Hp))).
+  split. {
+    rewrite in_map_iff.
+    exists (t', e).
+    auto.
+  }
+  eapply List.in_omap_1; eauto.
+  simpl.
+  destruct (prec_dec e' e). {
+    trivial.
+  }
+  contradiction.
 Qed.
 
-
-Lemma gen_tedges_spec:
-  forall e t s,
-  In (e, t) (gen_tedges s) <-> Impedes s e t.
+Let impeded_by_spec:
+  forall t e s,
+  In (e, t) (impeded_by s) <->
+  Impedes s e t.
 Proof.
-  intros.
-  split.
-  - apply in_gen_tedges_to_blocks.
-  - apply blocks_to_in_gen_tedges.
+  split; eauto.
 Qed.
-
-Module I := Project Map_EVT Set_TID.
 
 Let evt_eq_helper:
   forall k1 k2 : nat * nat, fst k1 = fst k2 /\ snd k1 = snd k2 -> k1 = k2.
@@ -637,9 +499,9 @@ Proof.
   simpl in *; auto.
 Qed.
 
-Definition to_impedes s := I.unproject evt_eq_helper (gen_tedges s).
+Definition to_impedes s := I.unproject evt_eq_helper (impeded_by s).
 
-Lemma impedes_total:
+Let impedes_total:
   forall (s:state),
   exists (i:impedes), I_of s i.
 Proof.
@@ -649,8 +511,7 @@ Proof.
   intros.
   split; intros.
   - apply I.unproject_spec in H; auto.
-    apply gen_tedges_spec in H; auto.
-  - apply gen_tedges_spec in H; auto.
+  - apply impeded_by_spec in H; auto.
     apply I.unproject_spec; auto.
 Qed.
 
@@ -665,3 +526,4 @@ Proof.
   unfold Deps_of.
   intuition.
 Qed.
+End Props.
